tests/defined/shadowing.c
@@ -1,0 +1,31 @@
+#include<stdio.h>
+
+int x;
+
+int main() {
+  if (x != 10) printf("ERROR 1\n");
+  {
+    int x = 11;
+    if (x != 11) printf("ERROR 2\n");
+    {
+      extern int x;
+      if (x != 10) printf("ERROR 3\n");
+    }
+  }
+  int *p;
+  {
+    static int y;
+    if (y != 0) printf("ERROR 4\n");
+    {
+      int y = 14;
+      if (y != 14) printf("ERROR 5\n");
+    }
+    p = &y;
+    y = 16;
+  }
+  if (*p != 16) printf("ERROR 6\n");
+  return 0;
+}
+
+int x = 10;
+int x;
